feat: towards unformalized algorithms

Cube/Simple/Basic.lean
@@ -1,8 +1,6 @@
 import Cube.Util
 import Cube.Context
 
-import Mathlib.Tactic.Linarith
-
 import Lean
 
 open Lean
@@ -12,21 +10,34 @@ namespace Cube.Simple
 inductive Ty where
 | nat
 | fun (pre : Ty) (image : Ty)
-deriving Repr, DecidableEq
+deriving Repr, DecidableEq, Inhabited, Hashable
+
+def Ty.telescope (ty : Ty) : Array Ty :=
+  go ty #[]
+where
+  go (ty : Ty) (acc : Array Ty) :=
+    match ty with
+    | .nat => acc.push .nat
+    | .fun t1 t2 => go t2 (acc.push t1)
+
+def Ty.ofTelescope (telescope : Array Ty) : Ty :=
+  telescope[:telescope.size - 1].foldr (init := telescope[telescope.size - 1]!) (fun arg acc => .fun arg acc)
 
 inductive Ast where
 | var (name : String)
 | const (name : String)
 | lam (var : String) (ty : Ty) (body : Ast)
 | app (func : Ast) (arg : Ast)
+deriving Repr
 
 inductive Expr where
 | bvar (idx : Nat)
 | fvar (name : FVarId)
-| lam (ty : Ty) (body : Expr) (orig : String)
+| lam (orig : String) (ty : Ty) (body : Expr)
 | const (name : String)
 | app (func : Expr) (arg : Expr)
-deriving Repr, DecidableEq
+deriving Repr, DecidableEq, Inhabited, Hashable
+
 abbrev TranslationEnv := List String
 
 def Ast.toExpr : Ast → TranslationEnv → Expr
@@ -36,14 +47,14 @@ def Ast.toExpr : Ast → TranslationEnv → Expr
   | none => .fvar ⟨name, 0⟩
 | const name, _ => .const name
 | app func arg, vs => .app (toExpr func vs) (toExpr arg vs)
-| lam x ty body, vs => .lam ty (toExpr body <| x :: vs) x
+| lam x ty body, vs => .lam x ty (toExpr body <| x :: vs)
 
 def Expr.toAst : Expr → TranslationEnv → Option Ast
 | bvar idx, vs => do
   let x ← vs[idx]?
   return .var x
 | fvar fvarId, _ => some <| .var fvarId.name
-| lam ty body name, vs => do
+| lam name ty body, vs => do
     let body ← toAst body <| name :: vs
     return .lam name ty body
 | const name, _ => some <| .const name
@@ -59,14 +70,15 @@ syntax stlcTy "→" stlcTy : stlcTy
 syntax "(" stlcTy ")" : stlcTy
 
 syntax ident : stlc
-syntax stlc:11 stlc:10 : stlc
+syntax num : stlc
+syntax stlc:10 stlc:11 : stlc
 syntax "λ " ident ":" stlcTy " . " stlc : stlc
 syntax "(" stlc ")" : stlc
 
 syntax "[stlcTy|" stlcTy "]" : term
 syntax "[stlcA|" stlc "]" : term
 syntax "[stlc|" stlc "]" : term
-
+#check String.Pos
 macro_rules
   | `([stlcTy| ℕ]) => `(Ty.nat)
   | `([stlcTy| $a → $b]) => `(Ty.fun [stlcTy| $a] [stlcTy| $b])
@@ -74,14 +86,18 @@ macro_rules
 
   | `([stlcA| $x:ident]) =>
     let strId := x.getId.toString
-    if strId.startsWith "@" then
-      `(Ast.const $(quote <| strId.drop 1))
+    let first := strId.get ⟨0⟩
+    if first.isUpper then
+      `(Ast.const $(quote <| strId))
     else
       `(Ast.var $(quote strId))
+  | `([stlcA| $n:num]) => `(Ast.const $(quote n.getNat.repr))
   | `([stlcA| λ $x : $ty . $b]) => `(Ast.lam $(quote x.getId.toString) [stlcTy| $ty]  [stlcA| $b])
   | `([stlcA| $f $x]) => `(Ast.app [stlcA| $f] [stlcA| $x])
   | `([stlcA| ($x)]) => `([stlcA| $x])
   | `([stlc| $t ]) => `(Ast.toExpr [stlcA| $t] [])
+
+#eval [stlcTy| (ℕ → ℕ → ℕ) → ℕ → ℕ] == (Ty.ofTelescope [stlcTy| (ℕ → ℕ → ℕ) → ℕ → ℕ].telescope)
 
 theorem Ast.toExpr_inv_toAst (a : Ast) (xs : List String) : Expr.toAst (Ast.toExpr a xs) xs = some a := by
   induction a generalizing xs with
@@ -103,9 +119,10 @@ theorem Ast.toExpr_inv_toAst (a : Ast) (xs : List String) : Expr.toAst (Ast.toEx
 
 theorem Ast.macro_correct (a : Ast) : Expr.toAst (Ast.toExpr a []) [] = some a := toExpr_inv_toAst a []
 
-example := [stlc| λ x : ℕ . (λ y : ℕ → ℕ . free y x)]
+#eval [stlc| λ x : ℕ . (λ y : ℕ → ℕ . (free y) x)]
 
 namespace Expr
+
 -- From I'm not a number I'm a free variable
 def abstract (expr : Expr) (target : FVarId) (idx : Nat := 0): Expr :=
   match expr with
@@ -115,7 +132,7 @@ def abstract (expr : Expr) (target : FVarId) (idx : Nat := 0): Expr :=
     else
       .fvar name
   | .app fn arg => .app (abstract fn target idx) (abstract arg target idx )
-  | .lam ty body orig => .lam ty (abstract body target (idx + 1)) orig
+  | .lam orig ty body => .lam orig ty (abstract body target (idx + 1))
   | .const name => .const name
   | .bvar idx => .bvar idx
 
@@ -127,133 +144,368 @@ def instantiate (expr : Expr) (image : Expr) (targetIdx : Nat := 0) : Expr :=
     else
       .bvar idx
   | .app fn arg => .app (instantiate fn image targetIdx ) (instantiate arg image targetIdx )
-  | .lam ty body orig => .lam ty (instantiate body image (targetIdx + 1)) orig
+  | .lam orig ty body => .lam orig ty (instantiate body image (targetIdx + 1))
   | .fvar name => .fvar name
   | .const name => .const name
 
-inductive FVarIn (fvarId : FVarId) : Expr → Prop where
-| fvarEq : FVarIn fvarId (.fvar fvarId)
-| appLeft (func arg : Expr) (h : FVarIn fvarId func) : FVarIn fvarId (.app func arg)
-| appRight (func arg : Expr) (h : FVarIn fvarId arg) : FVarIn fvarId (.app func arg)
-| lam (ty : Ty) (body : Expr) (h : FVarIn fvarId body) : FVarIn fvarId (.lam ty body orig)
+def substitute (expr : Expr) (fvarId : FVarId) (image : Expr) : Expr :=
+  expr.abstract fvarId |>.instantiate image
 
-def FreshIn (fvar : FVarId) (expr : Expr) := ¬ FVarIn fvar expr
-def Closed (expr : Expr) := ∀ fvar, FreshIn fvar expr
+abbrev Context := Cube.Context Ty
+abbrev Env := Cube.Env Ty
+abbrev Substitution := Cube.Substitution Expr
+abbrev SimpleT (m : Type → Type) := ReaderT Env (StateT Context (ExceptT String m))
+abbrev SimpleM := SimpleT Id
 
-inductive LocallyClosed : Expr → Prop where
-| const (name : String) : LocallyClosed (.const name)
-| fvar (fvarId : FVarId) : LocallyClosed (.fvar fvarId)
-| app (func arg : Expr) (closedFunc : LocallyClosed func) (closedArg : LocallyClosed arg) : LocallyClosed (.app func arg)
-| lam (ty : Ty) (body : Expr) (freeBody : FreshIn x body) (closedBody : LocallyClosed (abstract body x)) : LocallyClosed (.lam ty body orig)
+def getCtx : SimpleM Context := do return (← get)
+def getEnv : SimpleM Env := do return (← read)
+def SimpleM.run' (x : SimpleM α) (env : Env) (ctx : Context) : Except String α :=
+  x.run env |>.run' ctx
 
-inductive ClosedTo : Nat → Expr → Prop where
-| const (n : Nat) (name : String) : ClosedTo n (.const name)
-| bvar (idx m : Nat) (closed : idx < m): ClosedTo m (.bvar idx)
-| fvar (n : Nat) (fvarId : FVarId) : ClosedTo n (.fvar fvarId)
-| app (func arg : Expr) (closedFunc : ClosedTo n func) (closedArg : ClosedTo n arg) : ClosedTo n (.app func arg)
-| lam (closedBody : ClosedTo (n + 1) body) : ClosedTo n (.lam ty body orig)
+partial def infer (expr : Expr) : SimpleM Ty := do
+  match h:expr with
+  | .bvar idx => throw s!"Unbound variable index: {idx}"
+  | .app fn arg => 
+      if let .fun t1 t2 ← infer fn then
+        let t3 ← infer arg
+        if t1 = t3 then
+          return t2
+        else
+          throw s!"Arg type mismatch in {repr expr}, argument should have type {repr t1} but has type {repr t3}"
+      else
+        throw s!"Function type mismatch in {repr expr}, function should have function type"
+  | .lam _ t1 body =>
+    let newFVar := FVar.fresh (← getCtx)
+    let newBody := body.instantiate (.fvar newFVar)
+    let ctx ← getCtx
+    modify (fun ctx => ctx.insert newFVar t1)
+    try
+      let t2 ← infer newBody
+      return .fun t1 t2
+    finally
+      set ctx
+  | .fvar fvarId =>
+    if let some typ := (← getCtx).find? fvarId then
+      return typ
+    else
+      throw s!"FVarId: {repr fvarId} not found in context"
+  | .const name => 
+    if let some typ := (← getEnv).find? name then
+      return typ
+    else
+      throw s!"Constant: {name} not found in environment"
 
-abbrev LocallyClosed' (expr : Expr) := ClosedTo 0 expr
 
-abbrev _root_.Cube.WfExpr := { expr : Expr // LocallyClosed expr }
+partial def betaReduce (expr : Expr) : Expr :=
+  match expr with
+  | .app fn arg =>
+    let newArg := betaReduce arg
+    match fn with
+    | .lam _ _ body =>
+      let newBody := body.instantiate arg
+      betaReduce newBody
+    | _ => .app (betaReduce fn) newArg
+  | .lam orig t body => .lam orig t (betaReduce body)
+  | .bvar idx => .bvar idx
+  | .fvar fvarId => .fvar fvarId
+  | .const name => .const name
 
-theorem instantiate_abstract_self_eq (expr : Expr) (h : FreshIn target expr) : (expr.instantiate (.fvar target) i).abstract target i = expr := by
-  induction expr generalizing i with
-  | bvar =>
-    simp only [instantiate]
-    split <;> simp_all[abstract]
-  | fvar =>
-    simp only [instantiate, abstract]
-    split
-    next h2 =>
-      apply h
-      rw [h2]
-      apply FVarIn.fvarEq
-    next => rfl
-  | const => simp [abstract, instantiate]
-  | lam ty body orig bih =>
-    simp only [instantiate, abstract, lam.injEq, and_true, true_and]
-    apply bih
-    intro h2
-    apply h
-    apply FVarIn.lam
-    assumption
-  | app func arg fih aih =>
-    simp only [instantiate, abstract, app.injEq]
-    constructor
-    case left =>
-      apply fih
-      intro h2
-      apply h
-      apply FVarIn.appLeft
-      assumption
-    case right =>
-      apply aih
-      intro h2
-      apply h
-      apply FVarIn.appRight
-      assumption
+#eval betaReduce [stlc| (λ f : ℕ → ℕ. f 12) (λ x : ℕ. x)]
+#eval infer [stlc| (λ f : ℕ → ℕ. f 12) (λ x : ℕ. x)] |>.run' (Env.empty.insert "12" .nat) {}
+#eval betaReduce [stlc| (λ f : ℕ → ℕ. g (f 12)) (λ x : ℕ. x)]
+#eval infer [stlc| (λ f : ℕ → ℕ. g (f 12)) (λ x : ℕ. x)] |>.run' (Env.empty.insert "12" .nat) (Context.empty.insert ⟨"g", 0⟩ [stlcTy| ℕ → ℕ])
 
-theorem abstract_instantiate_self_eq' (expr : Expr) (h : ClosedTo i expr) : (expr.abstract target i).instantiate (.fvar target) i = expr := by
-  induction expr generalizing i with
-  | bvar =>
-    simp only [instantiate, ite_eq_right_iff]
-    intro h2
-    cases h
-    linarith
-  | const => simp [abstract, instantiate]
-  | fvar =>
-    simp only [abstract]
-    split <;> simp_all [instantiate]
-  | app func arg fih aih =>
-    simp only [abstract, instantiate, app.injEq]
-    cases h
-    constructor
-    case left => apply fih; assumption
-    case right => apply aih; assumption
-  | lam ty body orig ihb =>
-    simp only [abstract, instantiate, lam.injEq, true_and, and_true] at *
-    cases h
-    apply ihb
-    assumption
+def applySubst (subst : Substitution) (expr : Expr) : Expr :=
+  subst.toList.foldl (init := expr) (fun expr (fvarId, image) => expr.substitute fvarId image)
 
-  
-theorem LocallyClosed'.succ_closed_of_abstract_closed (h : ClosedTo i (abstract expr x i)) : ClosedTo (i + 1) expr := by
-  induction expr generalizing i with
-  | bvar =>
-    simp only [abstract] at h
-    cases h
-    apply ClosedTo.bvar
-    linarith
-  | fvar => apply ClosedTo.fvar
-  | const => apply ClosedTo.const
-  | app func arg fih aih =>
-    cases h
-    apply ClosedTo.app
-    case closedFunc => apply fih; assumption
-    case closedArg => apply aih; assumption
-  | lam ty body tih bih =>
-    cases h
-    apply ClosedTo.lam
-    case closedBody => apply bih; assumption 
+def lambdaLength (expr : Expr) (n : Nat := 0) : Nat :=
+  match expr with
+  | .lam _ _ body => lambdaLength body (n + 1)
+  | _ => n
 
-theorem LocallyClosed.iff_LocallyClosed' (h : LocallyClosed expr) : LocallyClosed' expr := by
-  induction h with
-  | const => apply ClosedTo.const
-  | fvar => apply ClosedTo.fvar
-  | app =>
-    apply ClosedTo.app
-    repeat assumption
-  | lam =>
-    apply ClosedTo.lam
-    case closedBody =>
-      apply LocallyClosed'.succ_closed_of_abstract_closed
-      repeat assumption
+def typeLength (ty : Ty) : Nat :=
+  match ty with
+  | .nat => 0
+  | .fun _ t2 => 1 + typeLength t2
 
-theorem abstract_instantiate_self_eq (expr : Expr) (h : LocallyClosed expr) : (expr.abstract target).instantiate (.fvar target) = expr := by
-  apply abstract_instantiate_self_eq'
-  apply LocallyClosed.iff_LocallyClosed'
-  assumption
+def getNthType! (ty : Ty) (idx : Nat) : Ty :=
+  match ty, idx with
+  | .nat, 0 => .nat
+  | .fun t1 _, 0 => t1
+  | .nat, _ + 1 => panic! "Invalid index"
+  | .fun _ t2, n + 1 => getNthType! t2 n
+
+-- TODO: I think this is a locally nameless anti pattern?
+def raiseIndices (expr : Expr) (n : Nat) : Expr :=
+  match expr with
+  | .app fn arg => .app (raiseIndices fn n) (raiseIndices arg n)
+  | .lam orig t body => .lam orig t (raiseIndices body n)
+  | .bvar idx => .bvar (idx + n)
+  | .fvar fvarId => .fvar fvarId
+  | .const name => .const name
+
+def etaExpand (expr : Expr) (ty : Ty) : Expr :=
+  -- TODO: Optimize, etaExpand is called from betaEtaNormalForm
+  -- which already computes lamLen and tyLen
+  let lamLen := lambdaLength expr
+  let tyLen := typeLength ty
+  if lamLen == tyLen then
+    expr
+  else
+    let relevantTy := getNthType! ty (tyLen - lamLen)
+    go expr relevantTy
+where
+  go (expr : Expr) (relevantTy : Ty) : Expr :=
+    match expr with
+    | .lam orig t body => .lam orig t (go body relevantTy)
+    | _ => .lam "eta" relevantTy (.app (raiseIndices expr 1) (.bvar 0))
+
+def betaEtaNormalForm (expr : Expr) (ty : Ty) : Expr :=
+  let betaNormalForm := betaReduce expr
+  let n := lambdaLength expr
+  let m := typeLength ty
+  let len := m - n
+  -- TODO: Optimize, we can also eta expand m - n at once
+  len.fold (init := betaNormalForm) (fun _ expr => etaExpand expr ty)
+
+-- TODO: These produce unbounded bvars...
+def lambdaTelescope (expr : Expr) : Array Ty × Expr :=
+  go expr #[]
+where
+  go (expr : Expr) (binders : Array Ty) : Array Ty × Expr :=
+    match expr with
+    | .lam _ t1 body => go body (binders.push t1)
+    | _ => (binders, expr)
+
+def abstractArgs (body : Expr) (args : Array Ty) : Expr :=
+  args.foldr (init := body) (fun ty body => .lam "abstract" ty body)
+
+def appTelescope (expr : Expr) : Array Expr × Expr :=
+  let (revArgs, remainder) := go expr #[]
+  (revArgs.reverse, remainder)
+where
+  go (expr : Expr) (args : Array Expr) : Array Expr × Expr :=
+    match expr with
+    | .app fn arg => go fn (args.push arg)
+    | _ => (args, expr)
+
+def mkApp (fn : Expr) (args : Array Expr) : Expr :=
+  args.foldl (init := fn) (fun fn arg => .app fn arg)
+
+#eval mkApp (.const "1") #[.const "2", .const "3"] == [stlc| (1 2) 3] 
+
+-- TODO: Maybe it is worth it to have a seperate data type for βη normalized exprs
+namespace Unify
+
+inductive Head where
+| const (name : String)
+| bvar (idx : Nat)
+| fvar (fvarId : FVarId)
+deriving DecidableEq, Hashable, Inhabited, Repr
+
+structure BetaEtaNormalExpr where
+  binder : Array Ty
+  head : Head
+  args : Array Expr
+deriving DecidableEq, Hashable, Inhabited, Repr
+
+def BetaEtaNormalExpr.ofNormalExpr (expr : Expr) : BetaEtaNormalExpr :=
+  let (binder, body) := lambdaTelescope expr
+  let (args, head) := appTelescope body
+  let head := match head with
+    | .const name => .const name
+    | .bvar idx => .bvar idx
+    | .fvar fvarId => .fvar fvarId
+    | _ => panic! "Not in correct normal form"
+  { binder, head, args }
+
+def BetaEtaNormalExpr.ofExpr (expr : Expr) (ty : Ty) : BetaEtaNormalExpr :=
+  .ofNormalExpr <| betaEtaNormalForm expr ty
+
+def Head.toExpr (head : Head) : Expr :=
+  match head with
+  | .const name => .const name
+  | .bvar idx => .bvar idx
+  | .fvar fvarId => .fvar fvarId
+
+def BetaEtaNormalExpr.toExpr (expr : BetaEtaNormalExpr) : Expr :=
+  let body := mkApp expr.head.toExpr expr.args
+  abstractArgs body expr.binder
+ 
+inductive Flexibility where
+| rigid
+| flexible
+
+def BetaEtaNormalExpr.flexibility (expr : BetaEtaNormalExpr) : Flexibility :=
+  match expr.head with
+  | .fvar .. => .flexible
+  | _ => .rigid
+
+theorem BetaEtaNormalExpr.False_of_rigid_fvar {expr : BetaEtaNormalExpr} (h1 : expr.flexibility = .rigid) (h2 : expr.head = .fvar fvarId) : False := by
+  unfold flexibility at h1
+  rw [h2] at h1
+  simp at h1
+
+def BetaEtaNormalExpr.headType (expr : BetaEtaNormalExpr) : SimpleM Ty := do
+  match expr.head with
+  | .const name => return (← read).find! name
+  | .fvar fvarId => return (← get).find! fvarId
+  | .bvar idx => return expr.binder.get! (expr.binder.size - idx)
+
+def inhabitant (ty : Ty) : Expr :=
+  match ty with
+  | .nat => .const "0"
+  | .fun t1 t2 => .lam "inhab" t1 (inhabitant t2)
+
+def BetaEtaNormalExpr.headFVarId (expr : BetaEtaNormalExpr) (h : expr.flexibility = .flexible) : FVarId :=
+  match h2:expr.head with
+  | .fvar fvarId => fvarId
+  | .bvar idx | .const name => by simp [flexibility, h2] at h
+
+def BetaEtaNormalExpr.applySubst (normalExpr : BetaEtaNormalExpr) (subst : Substitution) : SimpleM BetaEtaNormalExpr := do
+  let expr := normalExpr.toExpr
+  let substExpr := expr.applySubst subst
+  let ty ← infer substExpr
+  return BetaEtaNormalExpr.ofExpr substExpr ty 
+ 
+abbrev DisagreementPair := BetaEtaNormalExpr × BetaEtaNormalExpr
+abbrev DisagreementSet := HashSet DisagreementPair
+structure UnifyNode where
+  disagreement : DisagreementSet
+  substitution : Substitution
+
+def DisagreementPair.apply (pair : DisagreementPair) (subst : Substitution) : SimpleM DisagreementPair :=
+  return (← pair.fst.applySubst subst, ← pair.snd.applySubst subst)
+
+def DisagreementSet.apply (set : DisagreementSet) (subst : Substitution) : SimpleM DisagreementSet :=
+  set.foldM (init := HashSet.empty) (fun new pair => do return new.insert (← pair.apply subst))
+
+def UnifyNode.apply (node : UnifyNode) (subst : Substitution) : SimpleM UnifyNode := do
+  return ⟨← node.disagreement.apply subst, node.substitution.compose subst⟩
+
+-- https://www21.in.tum.de/teaching/sar/SS20/5.pdf
+partial def unify (e1 e2 : Expr) : SimpleM Substitution := do
+  let t1 ← infer e1 
+  let t2 ← infer e2
+  if t1 == t2 then
+    let e1Normal := BetaEtaNormalExpr.ofExpr e1 t1
+    let e2Normal := BetaEtaNormalExpr.ofExpr e2 t1
+    go [⟨HashSet.empty.insert (e1Normal, e2Normal), {}⟩]
+  else
+    throw "Types don't match"
+where
+  go (state : List UnifyNode) : SimpleM Substitution := do
+    match state with
+    | [] => throw "Gave up after exhaustive search"
+    | node :: rest =>
+      match ← simplify node with
+      | none => go rest
+      | some (.inl subst) => return subst
+      | some (.inr node) =>
+        match findMatcherTarget node.disagreement with
+        | some (lhs, rhs) =>
+          let candidates ← matcher lhs rhs
+          let newNodes ← candidates.mapM node.apply
+          go <| rest.append newNodes
+        | none => go <| rest.append [node]
+
+  simplify (node : UnifyNode) : SimpleM (Option (Substitution ⊕ UnifyNode)) := do
+    let mut newSet := HashSet.empty
+    let mut newSubst := node.substitution
+    for pair in node.disagreement do
+      match ← simplifyPair pair newSubst with
+      | none => return none
+      | some (.inl subst) => newSubst := subst
+      | some (.inr set) => newSet := newSet.merge set
+    if newSet.isEmpty then
+      return some <| .inl newSubst
+    else
+      return some <| .inr ⟨newSet, newSubst⟩
+
+  simplifyPair (pair : DisagreementPair) (subst : Substitution) : SimpleM (Option (Substitution ⊕ DisagreementSet)) := do
+    let lhs := pair.fst
+    let rhs := pair.snd
+    dbg_trace s!"{repr lhs} =?= {repr rhs}"
+    match hlflex:lhs.flexibility, hrflex:rhs.flexibility with
+    | .rigid, .rigid =>
+      dbg_trace s!"Rigid, Rigid"
+      if lhs.binder != rhs.binder || lhs.head != rhs.head then
+        return none
+      else
+        let newProblems := lhs.args.zip rhs.args
+        let folder := fun set (newLhs, newRhs) =>
+          let newLhs := BetaEtaNormalExpr.ofNormalExpr newLhs
+          let newRhs := BetaEtaNormalExpr.ofNormalExpr newRhs
+          let newPair := ⟨{newLhs with binder := lhs.binder.append newLhs.binder}, {newRhs with binder := rhs.binder.append newRhs.binder}⟩
+          dbg_trace s!"RR new: {repr newPair}"
+          set.insert newPair
+        let newDisagreements := newProblems.foldl (init := .empty) folder
+        return some <| .inr newDisagreements
+    | .flexible, .flexible =>
+      dbg_trace s!"Flex, Flex"
+      let lhsVal := inhabitant (← lhs.headType)
+      let rhsVal := inhabitant (← rhs.headType)
+      let subst := subst.insert (lhs.headFVarId hlflex) lhsVal
+        |>.insert (rhs.headFVarId hrflex) rhsVal
+      return some <| .inl subst
+    | .flexible, .rigid => dbg_trace s!"Flex, Rigid" return some <| .inr <| HashSet.empty.insert (lhs, rhs)
+    | .rigid, .flexible => dbg_trace s!"Rigid, Flex" return some <| .inr <| HashSet.empty.insert (rhs, lhs)
+
+  findMatcherTarget (set : DisagreementSet) : Option ({ e : BetaEtaNormalExpr // e.flexibility = .flexible} × { e : BetaEtaNormalExpr // e.flexibility = .rigid}) := do
+    for (lhs, rhs) in set do
+      match hlflex:lhs.flexibility, hrflex:rhs.flexibility with
+      -- simplify already turned .rigid, .flexible this way around
+      | .flexible, .rigid => return (⟨lhs, hlflex⟩, ⟨rhs, hrflex⟩)
+      | _, _ => pure ()
+    none
+
+  matcher (flex : { e : BetaEtaNormalExpr // e.flexibility = .flexible}) (rig : { e : BetaEtaNormalExpr // e.flexibility = .rigid}) : SimpleM (List Substitution) := do
+    let targetFVar := flex.val.headFVarId flex.property
+    let targetFVarTyTelescope := (← getCtx).find! targetFVar |>.telescope
+    match hhead:rig.val.head with
+    | .bvar idx => throw "not implemented" -- projection
+    | .const name =>
+      -- imitation
+      dbg_trace "imitation"
+      let mut candidates := []
+      let mut hs := #[]
+      let constTy := (← getEnv).find! name
+      let constTyTelescope := constTy.telescope
+      for hResTy in constTyTelescope[:constTyTelescope.size - 1] do
+        let hTyTelescope := targetFVarTyTelescope.set! (targetFVarTyTelescope.size - 1) hResTy
+        let hTy := Ty.ofTelescope hTyTelescope
+        let args := (hTyTelescope.size - 1).fold (init := #[]) (fun idx args => args.push (.bvar idx))
+        let hFVar ← FVar.freshM hTy
+        let hTerm := mkApp (.fvar hFVar) args
+        hs := hs.push hTerm
+      let replacer := abstractArgs (mkApp (.const name) hs) (targetFVarTyTelescope[:targetFVarTyTelescope.size - 1])
+      candidates := (Substitution.empty.insert targetFVar replacer) :: candidates
+      -- TODO: Projection
+      return candidates
+    | .fvar .. => nomatch BetaEtaNormalExpr.False_of_rigid_fvar rig.property hhead
+
+#eval show IO _ from do
+  let testPairs := #[
+    -- flexible, flexible
+    ([stlc| λ a : ℕ . f a], [stlc| λ b : ℕ . x], Env.empty, (Context.empty.insert ⟨"f", 0⟩ (.fun .nat .nat) |>.insert ⟨"x", 0⟩ .nat)),
+    -- rigid, rigid
+    ([stlc| λ f : ℕ → ℕ . f x], [stlc| λ g : ℕ → ℕ . g x], Env.empty, (Context.empty.insert ⟨"x", 0⟩ .nat)),
+    -- flexible, rigid const
+    ([stlc| λ x : ℕ . f x], [stlc| λ y : ℕ . 0], (Env.empty.insert "0" .nat), (Context.empty.insert ⟨"f", 0⟩ (.fun .nat .nat))),
+    ([stlc| λ x : ℕ . f x], [stlc| λ y : ℕ . C y], (Env.empty.insert "C" (.fun .nat .nat)), (Context.empty.insert ⟨"f", 0⟩ (.fun .nat .nat)))
+  ]
+  for (expr1, expr2, env, ctx) in testPairs do
+    let subst := unify expr1 expr2 |>.run' env ctx
+    match subst with
+    | .ok subst => 
+      let expr1' := expr1.applySubst subst |>.betaReduce
+      let expr2' := expr2.applySubst subst |>.betaReduce
+      IO.println s!"{repr expr1'}"
+      IO.println s!"{repr expr2'}"
+      IO.println ""
+    | .error e => IO.println s!"unification failure: {e} \n"
+
+end Unify
 
 end Expr
 
