Cube/Context.lean
@@ -5,7 +5,7 @@ namespace Cube
 structure FVarId where
   name : String
   id : Nat
-deriving Repr, DecidableEq
+deriving Repr, DecidableEq, Hashable
 
 def FVarId.toName (fvarId : FVarId) : Lean.Name :=
     .str (.num .anonymous fvarId.id) fvarId.name
@@ -15,37 +15,23 @@ instance : Ord FVarId where
 
 abbrev Env (Expr : Type u) := Std.RBMap String Expr (inferInstance : Ord String).compare
 abbrev Context (Expr : Type u)  := Std.RBMap FVarId Expr (inferInstance : Ord FVarId).compare
+abbrev Substitution (Expr : Type u)  := Std.RBMap FVarId Expr (inferInstance : Ord FVarId).compare
 
-def Env.get (env : Env Expr) (name : String) : Option Expr := env.find? name
-
-def Context.empty : Context Expr := Std.RBMap.empty
-
-def Context.update (ctx : Context Expr) (var : FVarId) (ty : Expr) : Context Expr :=
-  ctx.insert var ty
-
-def Context.get (ctx : Context Expr) (var : FVarId) : Option Expr := ctx.find? var
-
--- TODO: These should appear in std4 eventually
-theorem Context.get_empty (var : FVarId): Context.empty.get var = (none : Option Expr) := by
-  simp [Context.get, Std.RBMap.find?, empty, Std.RBMap.empty, Std.mkRBMap, Std.mkRBSet, Std.RBMap.findEntry?, Std.RBSet.findP?, Std.RBNode.find?, Option.map]
-
-theorem Context.get_update (ctx : Context Expr) (var : FVarId) (ty : Expr) : (ctx.update var ty).get var = some ty := by sorry
-
-theorem Context.get_update_irrelevant (ctx : Context Expr) (var1 var2 : FVarId) (ty : Expr) (h : var1 ≠ var2) : (ctx.update var1 ty).get var2 = ctx.get var2 := by sorry
+def Env.empty : Env Expr := {}
+def Context.empty : Context Expr := {}
+def Substitution.empty : Substitution Expr := {}
+def Substitution.compose (subst1 subst2 : Substitution Expr) : Substitution Expr :=
+  subst1.foldl (init := subst2) Std.RBMap.insert
 
 def FVar.fresh (ctx : Context Expr) : FVarId :=
   match ctx.max with
   | none => ⟨"_uniq", 0⟩
   | some (⟨_, idx⟩, _) => ⟨"_uniq", idx + 1⟩
 
-def FVar.freshM (ty : Expr) : StateM (Context Expr) FVarId := do
+def FVar.freshM {m : Type → Type} [MonadStateOf (Context Expr) m] [Monad m] (ty : Expr) : m FVarId := do
   let ctx ← get
   let new := FVar.fresh ctx
-  set (ctx.update new ty)
+  set (ctx.insert new ty)
   return new
-
-theorem FVar.fresh_is_fresh (ctx : Context Expr) : ctx.get (FVar.fresh ctx) = none := sorry
-theorem FVar.freshM_is_fresh (ctx : Context Expr) : ctx.get ((FVar.freshM ty).run' ctx) = none := by
-  simp [FVar.freshM, fresh_is_fresh]
 
 end Cube
